[lf] finish Imp

lf/Imp.v
@@ -463,13 +463,28 @@ Admitted.
     it is sound.  Use the tacticals we've just seen to make the proof
     as short and elegant as possible. *)
 
-Fixpoint optimize_0plus_b (b : bexp) : bexp
-  (* REPLACE THIS LINE WITH ":= _your_definition_ ." *). Admitted.
+Fixpoint optimize_0plus_b (b : bexp) : bexp :=
+  match b with
+  | BTrue => BTrue
+  | BFalse => BFalse
+  | BEq l r => BEq (optimize_0plus l) (optimize_0plus r)
+  | BNeq l r => BNeq (optimize_0plus l) (optimize_0plus r)
+  | BLe l r => BLe (optimize_0plus l) (optimize_0plus r)
+  | BGt l r => BGt (optimize_0plus l) (optimize_0plus r)
+  | BNot n => BNot (optimize_0plus_b n)
+  | BAnd l r => BAnd (optimize_0plus_b l) (optimize_0plus_b r)
+  end.
 
 Theorem optimize_0plus_b_sound : forall b,
   beval (optimize_0plus_b b) = beval b.
 Proof.
-  (* FILL IN HERE *) Admitted.
+  induction b ; 
+    simpl ;
+    try (rewrite optimize_0plus_sound; rewrite optimize_0plus_sound) ; 
+    try reflexivity.
+  - rewrite IHb. reflexivity.
+  - rewrite IHb1. rewrite IHb2. reflexivity.
+Qed.
 (** [] *)
 
 (** **** Exercise: 4 stars, standard, optional (optimize)
@@ -482,9 +497,38 @@ Proof.
     optimization and its correctness proof -- and build up
     incrementally to something more interesting.)  *)
 
-(* FILL IN HERE
+Fixpoint optimize_bnot (b : bexp) : bexp :=
+  match b with
+  | BTrue => BTrue
+  | BFalse => BFalse
+  | BEq l r => BEq l r
+  | BNeq l r => BNeq l r
+  | BLe l r => BLe l r
+  | BGt l r => BGt l r
+  | BNot l => 
+      match optimize_bnot l with
+      | BTrue => BFalse
+      | BFalse => BTrue
+      | BEq l r => BNeq l r
+      | BNeq l r => BEq l r
+      | BLe l r => BGt l r
+      | BGt l r => BLe l r
+      | BNot l => l
+      | BAnd l r => BNot (BAnd l r)
+      end
+  | BAnd l r => BAnd (optimize_bnot l) (optimize_bnot r)
+  end.
 
-    [] *)
+Theorem optimize_bnot_sound: forall b,
+  beval (optimize_bnot b) = beval b .
+Proof.
+  induction b ; try reflexivity.
+  - simpl. rewrite <- IHb.
+    destruct (optimize_bnot b); 
+      simpl; 
+      try (rewrite negb_involutive); try reflexivity.
+  - simpl. rewrite IHb1. rewrite IHb2. reflexivity.
+Qed.
 
 (* ================================================================= *)
 (** ** Defining New Tactics *)
@@ -847,14 +891,50 @@ Qed.
 
 Reserved Notation "e '==>b' b" (at level 90, left associativity).
 Inductive bevalR: bexp -> bool -> Prop :=
-(* FILL IN HERE *)
+  | E_BTrue : bevalR BTrue true
+  | E_BFalse : bevalR BFalse false
+  | E_BEq (a1 a2 : aexp) (v1 v2 : nat) :
+      a1 ==> v1 ->
+      a2 ==> v2 ->
+      BEq a1 a2 ==>b v1 =? v2
+  | E_BNeq (a1 a2 : aexp) (v1 v2 : nat) :
+      a1 ==> v1 ->
+      a2 ==> v2 ->
+      BNeq a1 a2 ==>b negb (v1 =? v2)
+  | E_BLe (a1 a2 : aexp) (v1 v2 : nat) :
+      a1 ==> v1 ->
+      a2 ==> v2 ->
+      BLe a1 a2 ==>b v1 <=? v2
+  | E_BGt (a1 a2 : aexp) (v1 v2 : nat) :
+      a1 ==> v1 ->
+      a2 ==> v2 ->
+      BGt a1 a2 ==>b negb (v1 <=? v2)
+  | E_BNot (e : bexp) (v : bool) :
+      e ==>b v -> BNot e ==>b negb v
+  | E_BAnd (e1 e2 : bexp) (v1 v2 : bool) :
+      e1 ==>b v1 ->
+      e2 ==>b v2 ->
+      BAnd e1 e2 ==>b v1 && v2
 where "e '==>b' b" := (bevalR e b) : type_scope
 .
 
 Lemma beval_iff_bevalR : forall b bv,
   b ==>b bv <-> beval b = bv.
 Proof.
-  (* FILL IN HERE *) Admitted.
+  intros. split.
+  - intros H. induction H ; 
+      simpl; 
+      try rewrite -> aeval_iff_aevalR in H; 
+      try rewrite -> aeval_iff_aevalR in H0;
+      subst; try constructor.
+  - generalize dependent bv.
+    induction b; intros; rewrite <- H; simpl; 
+    try (constructor; apply aeval_iff_aevalR; reflexivity).
+    + apply E_BNot. apply IHb. reflexivity.
+    + apply E_BAnd.
+      * apply IHb1. reflexivity.
+      * apply IHb2. reflexivity.
+Qed.
 (** [] *)
 
 End AExp.
@@ -1542,7 +1622,11 @@ Example ceval_example2:
     Z := 2
   ]=> (Z !-> 2 ; Y !-> 1 ; X !-> 0).
 Proof.
-  (* FILL IN HERE *) Admitted.
+  apply (E_Seq _ _ _ (X !-> 0)).
+  - apply E_Asgn. reflexivity.
+  - apply (E_Seq _ _ _ (Y !-> 1; X !-> 0));
+      apply E_Asgn; reflexivity.
+Qed.
 (** [] *)
 
 Set Printing Implicit.
@@ -1556,15 +1640,31 @@ Check @ceval_example2.
     which you can reverse-engineer to discover the program you should
     write.  The proof of that theorem will be somewhat lengthy. *)
 
-Definition pup_to_n : com
-  (* REPLACE THIS LINE WITH ":= _your_definition_ ." *). Admitted.
+Definition pup_to_n : com :=
+  <{Y := 0;
+    while X > 0 do
+      Y := Y + X;
+      X := X - 1
+    end}>.
 
 Theorem pup_to_2_ceval :
   (X !-> 2) =[
     pup_to_n
   ]=> (X !-> 0 ; Y !-> 3 ; X !-> 1 ; Y !-> 2 ; Y !-> 0 ; X !-> 2).
 Proof.
-  (* FILL IN HERE *) Admitted.
+  apply (E_Seq _ _ _ (Y !-> 0; X !-> 2)).
+  - apply E_Asgn. reflexivity.
+  - apply (E_WhileTrue _ (X !-> 1; Y !-> 2; Y !-> 0; X !-> 2)).
+    + reflexivity.
+    + apply (E_Seq _ _ _ (Y !-> 2; Y !-> 0; X !-> 2)).
+      * apply E_Asgn. reflexivity.
+      * apply E_Asgn. reflexivity.
+    + apply (E_WhileTrue _ (X !-> 0; Y !-> 3; X !-> 1; Y !-> 2; Y !-> 0; X !-> 2)).
+      * reflexivity.
+      * apply (E_Seq _ _ _ (Y !-> 3; X !-> 1; Y !-> 2; Y !-> 0; X !-> 2));
+          apply E_Asgn; reflexivity.
+      * apply E_WhileFalse. reflexivity.
+Qed.
 (** [] *)
 
 (* ================================================================= *)
@@ -1640,7 +1740,15 @@ Proof.
 
     State and prove a specification of [XtimesYinZ]. *)
 
-(* FILL IN HERE *)
+Theorem XtimesYinZ_spec: forall st x y st',
+  st X = x -> st Y = y ->
+  st =[ XtimesYinZ ]=> st' ->
+  st' Z = x * y.
+Proof.
+  intros st x y st' Ex Ey Heval.
+  inversion Heval. subst. simpl.
+  apply t_update_eq.
+Qed.
 
 (* Do not modify the following line: *)
 Definition manual_grade_for_XtimesYinZ_spec : option (nat*string) := None.
@@ -1659,7 +1767,11 @@ Proof.
       contradictory and so can be solved in one step with
       [discriminate]. *)
 
-  (* FILL IN HERE *) Admitted.
+  induction contra; try discriminate.
+  - injection Heqloopdef as Eb _.
+    rewrite Eb in H. simpl in H. discriminate.
+  - apply (IHcontra2 Heqloopdef).
+Qed.
 (** [] *)
 
 (** **** Exercise: 3 stars, standard (no_whiles_eqv)
@@ -1686,13 +1798,35 @@ Fixpoint no_whiles (c : com) : bool :=
     while loops.  Then prove its equivalence with [no_whiles]. *)
 
 Inductive no_whilesR: com -> Prop :=
- (* FILL IN HERE *)
+  | nw_skip : no_whilesR CSkip
+  | nw_asgn (s : string) (a : aexp) : no_whilesR (CAsgn s a)
+  | nw_seq (c1 c2 : com) : 
+      no_whilesR c1 ->
+      no_whilesR c2 ->
+      no_whilesR (CSeq c1 c2)
+  | nw_if (b : bexp) (c1 c2 : com) :
+      no_whilesR c1 ->
+      no_whilesR c2 ->
+      no_whilesR (CIf b c1 c2)
 .
 
 Theorem no_whiles_eqv:
   forall c, no_whiles c = true <-> no_whilesR c.
 Proof.
-  (* FILL IN HERE *) Admitted.
+  split.
+  - induction c; simpl.
+    + intros _. apply nw_skip.
+    + intros _. apply nw_asgn.
+    + intros H. rewrite andb_true_iff in H. destruct H as [H1 H2].
+      apply nw_seq. apply (IHc1 H1). apply (IHc2 H2).
+    + intros H. rewrite andb_true_iff in H. destruct H as [H1 H2].
+      apply nw_if. apply (IHc1 H1). apply (IHc2 H2).
+    + intros contra. discriminate.
+  - intros H. induction H;
+      simpl;
+      try (rewrite IHno_whilesR1; rewrite IHno_whilesR2);
+      reflexivity.
+Qed.
 (** [] *)
 
 (** **** Exercise: 4 stars, standard (no_whiles_terminating)
@@ -1702,7 +1836,21 @@ Proof.
 
     Use either [no_whiles] or [no_whilesR], as you prefer. *)
 
-(* FILL IN HERE *)
+Theorem no_whiles_terminating: forall st c,
+  no_whilesR c -> exists st', st =[ c ]=> st'.
+Proof.
+  intros st c H. generalize dependent st.
+  induction H; intros st.
+  + exists st. apply E_Skip.
+  + exists (s !-> aeval st a ; st). apply E_Asgn. reflexivity.
+  + destruct (IHno_whilesR1 st) as [s1 H1]. destruct (IHno_whilesR2 s1) as [s2 H2].
+    exists s2. apply (E_Seq _ _ _ s1). apply H1. apply H2.
+  + destruct (beval st b) eqn:Eb.
+    * destruct (IHno_whilesR1 st) as [st' H1].
+      exists st'. apply E_IfTrue. apply Eb. apply H1.
+    * destruct (IHno_whilesR2 st) as [st' H2].
+      exists st'. apply E_IfFalse. apply Eb. apply H2.
+Qed.
 
 (* Do not modify the following line: *)
 Definition manual_grade_for_no_whiles_terminating : option (nat*string) := None.
@@ -1774,7 +1922,15 @@ Inductive sinstr : Type :=
 Fixpoint s_execute (st : state) (stack : list nat)
                    (prog : list sinstr)
                  : list nat
-  (* REPLACE THIS LINE WITH ":= _your_definition_ ." *). Admitted.
+  := match prog, stack with
+    | [], _ => stack
+    | SPush n :: t, _ => s_execute st (n :: stack) t
+    | SLoad x :: t, _ => s_execute st (st x :: stack) t
+    | SPlus :: t, r :: l :: ss => s_execute st (l + r :: ss) t
+    | SMinus :: t, r :: l :: ss => s_execute st (l - r :: ss) t
+    | SMult :: t, r :: l :: ss => s_execute st (l * r :: ss) t
+    | _ :: t, _ => s_execute st stack t
+    end.
 
 Check s_execute.
 
@@ -1782,20 +1938,26 @@ Example s_execute1 :
      s_execute empty_st []
        [SPush 5; SPush 3; SPush 1; SMinus]
    = [2; 5].
-(* FILL IN HERE *) Admitted.
+Proof. reflexivity. Qed.
 
 Example s_execute2 :
      s_execute (X !-> 3) [3;4]
        [SPush 4; SLoad X; SMult; SPlus]
    = [15; 4].
-(* FILL IN HERE *) Admitted.
+Proof. reflexivity. Qed.
 
 (** Next, write a function that compiles an [aexp] into a stack
     machine program. The effect of running the program should be the
     same as pushing the value of the expression on the stack. *)
 
-Fixpoint s_compile (e : aexp) : list sinstr
-  (* REPLACE THIS LINE WITH ":= _your_definition_ ." *). Admitted.
+Fixpoint s_compile (e : aexp) : list sinstr :=
+  match e with
+  | ANum v => [SPush v]
+  | AId x => [SLoad x]
+  | APlus l r => s_compile l ++ s_compile r ++ [SPlus]
+  | AMinus l r => s_compile l ++ s_compile r ++ [SMinus]
+  | AMult l r => s_compile l ++ s_compile r ++ [SMult]
+  end.
 
 (** After you've defined [s_compile], prove the following to test
     that it works. *)
@@ -1803,7 +1965,7 @@ Fixpoint s_compile (e : aexp) : list sinstr
 Example s_compile1 :
   s_compile <{ X - (2 * Y) }>
   = [SLoad X; SPush 2; SLoad Y; SMult; SMinus].
-(* FILL IN HERE *) Admitted.
+Proof. reflexivity. Qed.
 (** [] *)
 
 (** **** Exercise: 3 stars, standard (execute_app) *)
@@ -1816,8 +1978,14 @@ Example s_compile1 :
 Theorem execute_app : forall st p1 p2 stack,
   s_execute st stack (p1 ++ p2) = s_execute st (s_execute st stack p1) p2.
 Proof.
-  (* FILL IN HERE *) Admitted.
-
+  intros st p1.
+  induction p1.
+  - simpl. intros p2 stack. reflexivity.
+  - intros p2 stack.
+    destruct stack.
+    + destruct a; simpl; apply IHp1.
+    + destruct stack; destruct a; simpl; apply IHp1.
+Qed.
 (** [] *)
 
 (** **** Exercise: 3 stars, standard (stack_compiler_correct) *)
@@ -1830,15 +1998,23 @@ Proof.
 Lemma s_compile_correct_aux : forall st e stack,
   s_execute st stack (s_compile e) = aeval st e :: stack.
 Proof.
-  (* FILL IN HERE *) Admitted.
+  intros st e.
+  induction e; 
+    simpl; intros stack;
+    try (
+      rewrite execute_app; rewrite IHe1;
+      rewrite execute_app; rewrite IHe2);
+    simpl; reflexivity.
+Qed.
 
 (** The main theorem should be a very easy corollary of that lemma. *)
 
 Theorem s_compile_correct : forall (st : state) (e : aexp),
   s_execute st [] (s_compile e) = [ aeval st e ].
 Proof.
-  (* FILL IN HERE *) Admitted.
-
+  intros st e.
+  rewrite s_compile_correct_aux. reflexivity.
+Qed.
 (** [] *)
 
 (** **** Exercise: 3 stars, standard, optional (short_circuit)
@@ -1858,9 +2034,28 @@ Proof.
     would _not_ be equivalent to the original, since it would make more
     programs terminate.) *)
 
-(* FILL IN HERE
+Fixpoint beval_sc (st : state) (b : bexp) : bool :=
+  match b with
+  | <{ true }> => true
+  | <{ false }> => false
+  | <{ a1 = a2 }> => aeval st a1 =? aeval st a2
+  | <{ a1 <> a2 }> => negb (aeval st a1 =? aeval st a2)
+  | <{ a1 <= a2 }> => aeval st a1 <=? aeval st a2
+  | <{ a1 > a2}> => negb (aeval st a1 <=? aeval st a2)
+  | <{ ~ b1 }> => negb (beval_sc st b1)
+  | <{ b1 && b2}> =>
+      match beval_sc st b1 with
+      | true => beval_sc st b2
+      | false => false
+      end
+  end.
 
-    [] *)
+Theorem beval_sc_correct: forall st b,
+  beval st b = beval_sc st b.
+Proof.
+  intros st.
+  induction b; simpl; reflexivity.
+Qed.
 
 Module BreakImp.
 (** **** Exercise: 4 stars, advanced (break_imp)
@@ -1982,7 +2177,38 @@ Reserved Notation "st '=[' c ']=>' st' '/' s"
 Inductive ceval : com -> state -> result -> state -> Prop :=
   | E_Skip : forall st,
       st =[ CSkip ]=> st / SContinue
-  (* FILL IN HERE *)
+  | E_Break : forall st,
+      st =[ CBreak ]=> st / SBreak
+  | E_asgn : forall st a n x,
+      aeval st a = n ->
+      st =[ x := a ]=> (x !-> n ; st) / SContinue
+  | E_IfTrue : forall st b c1 st' r c2,
+      beval st b = true ->
+      st=[ c1 ]=> st' / r ->
+      st =[ if b then c1 else c2 end ]=> st' / r
+  | E_IfFlase : forall st b c1 c2 st' r,
+      beval st b = false ->
+      st=[ c2 ]=> st' / r ->
+      st =[ if b then c1 else c2 end ]=> st' / r
+  | E_Seq1 : forall st c1 c2 st',
+      st=[ c1 ]=> st' / SBreak ->
+      st=[ c1 ; c2 ]=> st' / SBreak
+  | E_Seq2 : forall st c1 st1 c2 st2 r,
+      st=[ c1 ]=> st1 / SContinue ->
+      st1=[ c2 ]=> st2 / r ->
+      st=[ c1 ; c2 ]=> st2 / r
+  | E_WhileFalse : forall st b c,
+      beval st b = false ->
+      st =[ while b do c end ]=> st / SContinue
+  | E_WhileBreak : forall st b c st',
+      beval st b = true ->
+      st =[ c ]=> st' / SBreak ->
+      st =[ while b do c end ]=> st' / SContinue
+  | E_WhileTrue : forall st b c st' st'' r,
+      beval st b = true ->
+      st =[ c ]=> st' / SContinue ->
+      st' =[ while b do c end ]=> st'' / r ->
+      st =[ while b do c end ]=> st'' / SContinue
 
   where "st '=[' c ']=>' st' '/' s" := (ceval c st s st').
 
@@ -1992,33 +2218,46 @@ Theorem break_ignore : forall c st st' s,
      st =[ break; c ]=> st' / s ->
      st = st'.
 Proof.
-  (* FILL IN HERE *) Admitted.
+  intros.
+  inversion H.
+  - subst. inversion H5. reflexivity.
+  - inversion H2.
+Qed.
 
 Theorem while_continue : forall b c st st' s,
   st =[ while b do c end ]=> st' / s ->
   s = SContinue.
 Proof.
-  (* FILL IN HERE *) Admitted.
+  intros.
+  inversion H; reflexivity.
+Qed.
 
 Theorem while_stops_on_break : forall b c st st',
   beval st b = true ->
   st =[ c ]=> st' / SBreak ->
   st =[ while b do c end ]=> st' / SContinue.
 Proof.
-  (* FILL IN HERE *) Admitted.
+  intros.
+  apply E_WhileBreak. apply H. apply H0.
+Qed.
 
 Theorem seq_continue : forall c1 c2 st st' st'',
   st =[ c1 ]=> st' / SContinue ->
   st' =[ c2 ]=> st'' / SContinue ->
   st =[ c1 ; c2 ]=> st'' / SContinue.
 Proof.
-  (* FILL IN HERE *) Admitted.
+  intros.
+  apply E_Seq2 with (st1 := st').
+  apply H. apply H0.
+Qed.
 
 Theorem seq_stops_on_break : forall c1 c2 st st',
   st =[ c1 ]=> st' / SBreak ->
   st =[ c1 ; c2 ]=> st' / SBreak.
 Proof.
-  (* FILL IN HERE *) Admitted.
+  intros.
+  apply E_Seq1. apply H.
+Qed.
 (** [] *)
 
 (** **** Exercise: 3 stars, advanced, optional (while_break_true) *)
@@ -2027,7 +2266,16 @@ Theorem while_break_true : forall b c st st',
   beval st' b = true ->
   exists st'', st'' =[ c ]=> st' / SBreak.
 Proof.
-(* FILL IN HERE *) Admitted.
+  intros.
+  remember (<{ while b do c end }>) as c'.
+  induction H ; try discriminate Heqc'.
+  - injection Heqc' as Eb Ec. rewrite Eb in H.
+    rewrite H in H0. discriminate H0.
+  - injection Heqc' as Eb Ec. subst.
+    exists st. apply H1.
+  - injection Heqc' as Eb Ec. subst.
+    apply IHceval2. reflexivity. apply H0.
+Qed.
 (** [] *)
 
 (** **** Exercise: 4 stars, advanced, optional (ceval_deterministic) *)
@@ -2036,7 +2284,58 @@ Theorem ceval_deterministic: forall (c:com) st st1 st2 s1 s2,
      st =[ c ]=> st2 / s2 ->
      st1 = st2 /\ s1 = s2.
 Proof.
-  (* FILL IN HERE *) Admitted.
+  intros c st st1 st2 s1 s2 H1. 
+  generalize dependent s2. generalize dependent st2.
+  induction H1.
+  - intros st2 s2 H. inversion H.
+    split; reflexivity.
+  - intros st2 s2 H. inversion H.
+    split; reflexivity.
+  - intros st2 s2 H2. inversion H2.
+    split.
+    + rewrite H in H6. rewrite H6. reflexivity.
+    + reflexivity.
+  - intros st'' s2 H2. inversion H2.
+    + subst. apply IHceval. apply H9.
+    + rewrite H8 in H. discriminate H.
+  - intros st'' s2 H2. inversion H2.
+    + rewrite H8 in H. discriminate H.
+    + subst. apply IHceval. apply H9.
+  - intros st2 s2 H2.
+    inversion H2.
+    + subst. apply IHceval. apply H6.
+    + subst. apply IHceval in H3. destruct H3 as [_ contra].
+      discriminate contra.
+  - intros st'' s2 H2.
+    inversion H2.
+    + subst. apply IHceval1 in H5. destruct H5 as [_ contra].
+      discriminate contra.
+    + subst. apply IHceval2.
+      apply IHceval1 in H1. destruct H1 as [E13 _]. rewrite E13.
+      apply H6.
+  - intros st2 s2 He.
+    inversion He.
+    + split; reflexivity.
+    + rewrite H2 in H. discriminate H.
+    + rewrite H2 in H. discriminate H.
+  - intros st2 s2 He.
+    inversion He.
+    + subst. rewrite H6 in H. discriminate H.
+    + subst. split.
+      * apply IHceval in H7. destruct H7 as [E _]. apply E.
+      * reflexivity.
+    + subst. 
+      apply IHceval in H4. destruct H4 as [_ contra]. discriminate contra.
+  - intros st2 s2 He.
+    inversion He; subst.
+    + rewrite H5 in H. discriminate H.
+    + apply IHceval1 in H6. destruct H6 as [_ contra]. discriminate contra.
+    + split.
+      * apply IHceval1 in H3. destruct H3 as [Est' _].
+        rewrite <- Est' in H7. apply IHceval2 in H7. destruct H7 as [E _].
+        apply E.
+      * reflexivity.
+Qed.    
 
 (** [] *)
 End BreakImp.
